# Copyright 2016 ITEA 12004 SEAS Project.
# 
# Licensed under the Apache License, Version 2.0 (the "License");
# you may not use this file except in compliance with the License.
# You may obtain a copy of the License at
# 
#      http://www.apache.org/licenses/LICENSE-2.0
# 
# Unless required by applicable law or agreed to in writing,
# distributed under the License is distributed on an "AS IS" BASIS,
# WITHOUT WARRANTIES OR CONDITIONS OF ANY KIND, either express or implied.
# See the License for the specific language governing permissions and
# limitations under the License.

@prefix rdf: <http://www.w3.org/1999/02/22-rdf-syntax-ns#> .
@prefix owl: <http://www.w3.org/2002/07/owl#> .
@prefix rdfs: <http://www.w3.org/2000/01/rdf-schema#> .
@prefix xsd: <http://www.w3.org/2001/XMLSchema#> .
@prefix dcterms: <http://purl.org/dc/terms/> .
@prefix vann: <http://purl.org/vocab/vann/> .
@prefix voaf: <http://purl.org/vocommons/voaf#> .
@prefix vs: <http://www.w3.org/2003/06/sw-vocab-status/ns#> .
@prefix cc: <http://creativecommons.org/ns#>.
@prefix foaf: <http://xmlns.com/foaf/0.1/>.
@prefix ifc: <http://www.buildingsmart-tech.org/ifcOWL/IFC2X3_TC1#>. #IFC owl ontology
@prefix fiemser:<http://sites.google.com/site/smartappliancesproject/ontologies/fiemser#>. #Fiemser building ontology
@prefix saref: <http://ontology.tno.nl/saref#>. #SAREF smart building appliances ontology
@prefix gbxml:<http://www.gbxml.org/schema#>.     #GBXML XML schema

@prefix seas: <https://w3id.org/seas/>.
@base <https://w3id.org/seas/>.

voaf:Vocabulary a owl:Class .
dcterms:title a owl:AnnotationProperty .
dcterms:description a owl:AnnotationProperty .
dcterms:issued a owl:AnnotationProperty .
dcterms:modified a owl:AnnotationProperty .
dcterms:creator a owl:AnnotationProperty .
dcterms:contributor a owl:AnnotationProperty .
cc:license a owl:AnnotationProperty .
vann:preferredNamespacePrefix a owl:AnnotationProperty .
vann:preferredNamespaceUri a owl:AnnotationProperty .
vs:term_status a owl:AnnotationProperty .
foaf:Person a owl:Class .
foaf:name a owl:DatatypeProperty .



seas:BuildingOntology rdf:type voaf:Vocabulary , owl:Ontology ;
  dcterms:title "SEAS-BuildingOntology ontology"@en ;
  dcterms:description "The Seas Building BIM related vocabulary for the ITEA SEAS (Smart Energy Aware Systems) project. This ontology is targeted for defining structure of buildings (or more general facilities) and zones related to control and measurment with links to various BIM (Building Information Model) related standards."@en ;
  dcterms:issued "2016-01-26"^^xsd:date ;
  dcterms:modified "2016-05-26"^^xsd:date ;
  dcterms:creator <http://www.vtt.fi/JarmoKalaoja> ;
  dcterms:contributor <http://www.maxime-lefrancois.info/me#> ;
  cc:license <https://www.apache.org/licenses/LICENSE-2.0> ;
  vann:preferredNamespacePrefix "seas" ;
  vann:preferredNamespaceUri <https://w3id.org/seas/> ;  
  owl:versionIRI <https://w3id.org/seas/BuildingOntology-0.9> ;
  owl:versionInfo "v0.9" .

#General measurement and control concepts that are needed this could be linked to connection point ontology
seas:Site a owl:Class ;
  rdfs:label "Site"@en ;
  rdfs:comment "Site is a a specific locale with associated information describing its scope and context."@en ;
  rdfs:subClassOf seas:Entity;
  vs:term_status "testing" ;
  rdfs:isDefinedBy seas:BuildingOntology.  
  
seas:Zone a owl:Class ;
  rdfs:label "Zone"@en ;
  rdfs:comment "A general aggregation of administration, control, monitoring or measurement."@en ;
  rdfs:subClassOf seas:System;
  vs:term_status "testing" ;
  rdfs:isDefinedBy seas:BuildingOntology.      

seas:mesurementPointOf a owl:ObjectProperty;
  rdfs:label "measurementPointOf"@en ;
  rdfs:comment "Specifies scope of administration, control or mesurement. Mainly either PointOfControl and PointOfMeasurment."@en ;
  rdfs:subPropertyOf seas:connectionPointOf;
  rdfs:domain seas:ConnectionPoint; 
  rdfs:range seas:Zone;
  vs:term_status "testing" ;
  rdfs:isDefinedBy seas:BuildingOntology . 
  
seas:controlPointOf a owl:ObjectProperty;
  rdfs:label "controlPointOf"@en ;
  rdfs:comment "Specifies scope of administration, control or mesurement. Mainly either PointOfControl and PointOfMeasurment."@en ;
  rdfs:subPropertyOF seas:connectionPointOf;
  rdfs:domain seas:ConnectionPoint; 
  rdfs:range seas:Zone;
  vs:term_status "testing" ;
  rdfs:isDefinedBy seas:BuildingOntology .   
  
seas:PointOfControl a owl:Class ;
  rdfs:label "PointOfControl"@en ;
  rdfs:comment "Access role associated with controlling a specific zone"@en ;
  rdfs:subClassOf seas:ConnectionPoint;
  vs:term_status "testing" ;
  rdfs:isDefinedBy seas:BuildingOntology.    

seas:PointOfMeasurement a owl:Class ;
  rdfs:label "PointOfMeasurement"@en ;
  rdfs:comment "Access role of measurement information associated with a specific zone"@en ;
  rdfs:subClassOf seas:ConnectionPoint;
  vs:term_status "testing" ;
  rdfs:isDefinedBy seas:BuildingOntology.      


#These simplify defining relations between  connection points when we do not know the  underlying system connecitons  
seas:subMeasurement a owl:ObjectProperty; 
  rdfs:comment "The measurement in subMeasurement is contained in the value of higher level measurement"@en ;
  rdfs:subPropertyOf seas:contains;
  rdfs:domain seas:PointOfMeasurement;  
  rdfs:range seas:PointOfMeasurement;
  vs:term_status "testing" ;
  rdfs:isDefinedBy seas:BuildingOntology .     
  
seas:subControl a owl:ObjectProperty;
  rdfs:comment "Controlling the control point in subControl is already handled by the higher level control point."@en ;
  rdfs:subPropertyOf seas:contains;
  rdfs:domain seas:PointOfControl;
  rdfs:range seas:PointOfControl;
  vs:term_status "testing" ;
  rdfs:isDefinedBy seas:BuildingOntology .  
 
#Building structure core concepts  
#Building structure, seas does not define separate parameters quantitites such as coordinates or volumes
#Those can be defined as an an seas:Evaluation 
seas:SiteOfBuilding a owl:Class ;
  rdfs:label "SiteOfBuilding"@en ;
  rdfs:comment "Building site is a locale containing one or more separate buildings."@en ;
  rdfs:subClassOf seas:Site, seas:BuildingSpatialStructure;
  rdf:seeAlso ifc:Site;  
  vs:term_status "testing" ;
  rdfs:isDefinedBy seas:BuildingOntology.   

seas:ZoneOfBuilding a owl:Class ;
  rdfs:label "ZoneOfBuilding"@en ;
  rdfs:comment "An area of administration, control, monitoring or measurement inside a building."@en ;
  rdfs:subClassOf seas:Zone;
    rdfs:subClassOf [
      rdf:type owl:Restriction ;
      owl:allValuesFrom [
          rdf:type owl:Class ;
          owl:unionOf (
              seas:BuildingSpace 
			  seas:BuildingSurface 
			  seas:BuildingSystem 
			  seas:BuildingItem 
            ) ;
        ] ;
      owl:onProperty seas:contains ;
    ] ;
  vs:term_status "testing" ;
  rdf:seeAlso fiemser:BuildingZone, fiemser:BuildingPartition;
  rdfs:isDefinedBy seas:BuildingOntology.   

seas:Construction a owl:Class ;
  rdfs:label "Construction"@en ;
  rdfs:comment "Constructions are structures connected with the ground which are made of construction materials and components and/or for which construction work is carried out."@en ;
  rdfs:subClassOf seas:PhysicalEntity;
  vs:term_status "testing" ;
  rdfs:isDefinedBy seas:BuildingOntology.  

seas:CivilEngineeringWork a owl:Class ;
  rdfs:label "CivilEngnineeringWork"@en ;
  rdfs:comment "Civil engineering works are all constructions not classified under buildings : railways, roads, bridges, highways, airport runways, dams etc."@en ;
  rdfs:subClassOf seas:Construction;
  rdf:seeAlso ifc:Building, fiemser:Building;
  vs:term_status "testing" ;
  rdfs:isDefinedBy seas:BuildingOntology.  

# Building and its quantities

seas:Building a owl:Class ;
  rdfs:label "Building"@en ;
  rdfs:comment "Buildings are roofed constructions which can be used separately, have been built for permanent purposes, can be entered by persons and are suitable or intended for protecting persons, animals or objects."@en ;
  rdfs:subClassOf seas:BuildingSpatialStructure, seas:Construction;
  rdf:seeAlso ifc:Building, fiemser:Building;
  vs:term_status "testing" ;
  rdfs:isDefinedBy seas:BuildingOntology.  

seas:nominalEnergyConsumption a owl:ObjectProperty , owl:FunctionalProperty ;
  rdfs:label "nominal energy consumption"@en ;
  rdfs:label "ominaisenergiankulutus"@fi ;  
  rdfs:comment "Energy consumption of a building per gross floor area."@en ;
  rdfs:subPropertyOf seas:hasProperty ;
  rdfs:domain seas:PowerSystem ;
  rdfs:range seas:PowerPerAreaProperty ;
  vs:term_status "testing" ;
  rdfs:isDefinedBy seas:BuildingOntology. 

# Building and its quantities

seas:BuildingStorey a owl:Class ;
  rdfs:label "BuildingStorey"@en ;
  rdfs:comment "The storey represents a (nearly) horizontal aggregation of spaces that are vertically bound"@en;
  rdfs:subClassOf seas:BuildingSpatialStructure;
  vs:term_status "testing" ;
  rdf:seeAlso ifc:BuildingStorey;  
  rdfs:isDefinedBy seas:BuildingOntology.    
  
seas:BuildingRelated a owl:Class ; #From saref
  rdfs:label "BuildingRelated"@en ;
  rdfs:comment "Is a category that includes devices and systems as described by building related data models, such as FIEMSER "@en ;
  rdfs:subClassOf seas:DeviceCategory;
  rdfs:seeAlso saref:BuildingRelated;
  vs:term_status "testing" ;
  rdfs:isDefinedBy seas:BuildingOntology.      
  
seas:BuildingSpatialStructure a owl:Class ;
  rdfs:label "BuildingSpatialStructure"@en ;
  rdfs:comment "A man made structure with spatial properties"@en ;
  rdfs:subClassOf seas:BuildingSpace; 
  vs:term_status "testing" ;
  rdf:seeAlso ifc:IfcSpatialStructureElementType;
  rdfs:isDefinedBy seas:BuildingOntology.  

# building space 

seas:BuildingSpace a owl:Class ;
  rdfs:label "BuildingSpace"@en ;
  rdfs:comment "A Space is a 3D volume bounded by surfaces. According to the FIEMSER definition, a building space in SAREF defines the physical spaces of the building. A building space contains building items such as devices. "@en ;
  rdfs:subClassOf seas:PhysicalEntity; 
  vs:term_status "testing" ;
  rdf:seeAlso gbxml:BuildingSpace;    
  rdfs:isDefinedBy seas:BuildingOntology.  

seas:GrossFloorArea a owl:Class; 
  rdfs:label "GrossFloorArea"@en ;
  rdfs:comment "Gross floor area is generally defined by the area within the perimeter of the walls bounding the space."@en ;
  rdfs:subClassOf seas:Area;
  vs:term_status "testing" ;
  rdfs:isDefinedBy seas:BuildingOntology .  




seas:isAdjacentToSpace a owl:ObjectProperty;
  rdfs:label "isAdjacentToSpace"@en ;
  rdfs:comment "Surface is adjacent to a building space (or room)."@en ;
  rdfs:domain seas:BuildingSurface;
  rdfs:range seas:BuildingSpace;
  vs:term_status "testing" ;
  rdfs:isDefinedBy seas:BuildingOntology . 
  
seas:BuildingSurface a owl:Class ;
  rdfs:label "BuildingSurface"@en ;
  rdfs:comment "Surfaces such as surface of a wall element that encloses a space. In GbXML a surface can consist of several surfaces."@en ;
  rdfs:subClassOf seas:PhysicalEntity;
  vs:term_status "testing" ;
  rdfs:seeAlso gbxml:Surface;
  rdfs:isDefinedBy seas:BuildingOntology.  

seas:hasOpening a owl:ObjectProperty;
  rdfs:comment "hasOpening"@en ;
  rdfs:subPropertyOf seas:isPartOf;
  rdfs:domain seas:BuildingSurface;
  rdfs:range seas:SurfaceOpening;
  vs:term_status "testing" ;
  rdfs:isDefinedBy seas:BuildingOntology .   
  
seas:SurfaceOpening a owl:Class ;
  rdfs:label "SurfaceOpening"@en ;
  rdfs:comment "A opening in a surface such as window or door"@en ;
  rdfs:subClassOf seas:PhysicalEntity;
  vs:term_status "testing" ;
  rdfs:isDefinedBy seas:BuildingOntology.

seas:BuildingItem a owl:Class ; 
  rdfs:label "BuildingItem"@en ;
  rdfs:comment "A generalization of all the objects contained in building spaces that can have an unique location"@en ;
  owl:unionOf(seas:Device seas:Resident seas:Furnishing);
  vs:term_status "testing" ;
  rdfs:isDefinedBy seas:BuildingOntology.
  
seas:BuildingSystem a owl:Class ;
  rdfs:label "BuildingSystem"@en ;
  rdfs:comment "Any system not directly identifiable as a single building item inside building. It can contains several BuildingItems"@en ;
  rdfs:subClassOf seas:System;
  vs:term_status "testing" ;
  rdfs:isDefinedBy seas:BuildingOntology.      
  
#A few more specific terms mainly to help the user  
#GbXML defines a more specific types (such as interior wall) for these


seas:BuildingPartition a owl:Class ;
  rdfs:label "BuildingPartition"@en ;
  rdfs:comment "A collection of secific (restriction to be added) rooms such as apartement or wing."@en ;
  rdfs:subClassOf seas:ZoneOfBuilding;
  vs:term_status "testing" ;
  rdfs:isDefinedBy seas:BuildingOntology.   

seas:Room a owl:Class ;
  rdfs:label "Room"@en ;
  rdfs:comment "A room in a building space enclosed by surfaces, this could also be modelled as role of space, not subclass of the space itself."@en ;
  rdfs:subClassOf seas:BuildingSpace, seas:Area ;
  vs:term_status "testing" ;
  rdfs:isDefinedBy seas:BuildingOntology.   
  
seas:Wall a owl:Class ;
  rdfs:label "Wall"@en ;
  rdfs:comment "A Wall is (tilted more than 60 percent) vertical surface could be divided to interior, exterior and underground wall"@en ;
  rdfs:subClassOf seas:BuildingSurface;
  vs:term_status "testing" ;
  rdfs:isDefinedBy seas:BuildingOntology.    
  
seas:Floor a owl:Class ;
  rdfs:label "Floor"@en ;
  rdfs:comment "A floor is a upwards tilted horzontal surface, could be divided to interior, exposed (outside) or raised flooor."@en ;
  rdfs:subClassOf seas:BuildingSurface;
  vs:term_status "testing" ;
  rdfs:isDefinedBy seas:BuildingOntology.    

seas:Ceiling a owl:Class ;
  rdfs:label "Ceiling"@en ;
  rdfs:comment "Ceiling is a downwards tilted horizontal surface"@en ;
  rdfs:subClassOf seas:BuildingSurface;
  vs:term_status "testing" ;
  rdfs:isDefinedBy seas:BuildingOntology.    
  
seas:Roof a owl:Class ;
  rdfs:label "Roof"@en ;
  rdfs:comment "A roof upwards tilted surface tilted up part of upper envelope of building."@en ;
  rdfs:subClassOf seas:BuildingSurface;
  vs:term_status "testing" ;
  rdfs:isDefinedBy seas:BuildingOntology.      
      
seas:Door a owl:Class ;
  rdfs:label "Door"@en ;
  rdfs:comment "A door opening in a wall use for access between spaces."@en ;
  rdfs:subClassOf seas:SurfaceOpening;
  vs:term_status "testing" ;
  rdfs:isDefinedBy seas:BuildingOntology.     

seas:Window a owl:Class ;
  rdfs:label "Window"@en ;
  rdfs:comment "A window is a typically opaque opening not used as access between spaces."@en ;
  rdfs:subClassOf seas:SurfaceOpening;
  vs:term_status "testing" ;
  rdfs:isDefinedBy seas:BuildingOntology.     

#Different types entities of interest inside building that are not part of it 
    
seas:Furnishing a owl:Class ; 
  rdfs:label "Furnishing"@en ;
  rdfs:comment "Other things such as furniture, decorations and other possibly movable articles that are typically not devices"@en ;
  rdfs:subClassOf seas:PhysicalEntity;
  vs:term_status "testing" ;
  rdf:seeAlso ifc:IfcFurnishingElement;
  rdfs:isDefinedBy seas:BuildingOntology.     

seas:Resident a owl:Class ;
  rdfs:label "Resident"@en ;
  rdfs:comment "A resident of a building (might include also pets?)"@en ;
  rdfs:subClassOf seas:Role;
  vs:term_status "testing" ;
  rdfs:isDefinedBy seas:BuildingOntology. 

#To be moved to external vocabulary  
seas:hasComfortProfile a owl:ObjectProperty ;
  rdfs:label "hasComfortProfile"@en ;
  rdfs:comment "Shortcut for linking comfort profile settings for typically the resident but is open to other roles such as visitors or building owner."@en ;
  rdfs:domain seas:Role;
  rdfs:range seas:ComfortProfile;
  vs:term_status "testing" ;
  rdfs:isDefinedBy seas:BuildingOntology.  
  
seas:ComfortProfile a owl:Class ;
  rdfs:label "ComfortProfile"@en ;
  rdfs:comment "Comfort profile settings for the resident is defined as evaluations (a seas:profile is an evaluation). The comfortprofile is related to a room or other space with its featureOfInterest. The generatedBy links to activity that produced it."@en ;
  rdfs:subClassOf seas:Profile;
  vs:term_status "testing" ;
  rdfs:isDefinedBy seas:BuildingOntology.   

 
#Building categories based on its energy efficiency related to its insulation etc.
#The actual values for classes depend on the country specific regulations and geographical location

seas:NormHouse a owl:Class ; 
  rdfs:label "NormHouse"@en ;
  rdfs:label "Normitalo"@fi ;  
  rdfs:comment "A building fulfilling the minimal criteria for energy efficiency."@en ;
  rdfs:subClassOf seas:Building;
  vs:term_status "testing" ;
  rdfs:isDefinedBy seas:BuildingOntology.   

seas:LowEnergyHouse a owl:Class ;
  rdfs:label "LowEnergyHouse"@en ;
  rdfs:label "Matalaenergiatalo"@fi ;  
  rdfs:comment "A house typically consuming half the energy than a norm house."@en ;
  rdfs:subClassOf seas:Building;
  vs:term_status "testing" ;
  rdfs:isDefinedBy seas:BuildingOntology.     

seas:PassiveHouse a owl:Class ;
  rdfs:label "PassiveHouse"@en ;
  rdfs:label "Passiivitalo"@fi ;  
  rdfs:comment "A house typically consuming a quater of the energy than a norm house."@en ;
  rdfs:subClassOf seas:Building;
  vs:term_status "testing" ;
  rdfs:isDefinedBy seas:BuildingOntology.      

#Building categorization based on its net energy efficiency  
seas:ZeroEnergyBuilding a owl:Class ;
  rdfs:label "ZeroEnergyBuilding"@en ;
  rdfs:label "Nollaenergiatalo"@fi ;  
  rdfs:comment "A net zero-energy building (ZEB) is a building that over a year does not use more energy than it generates. "@en ;
  rdfs:subClassOf seas:Building;
  vs:term_status "testing" ;
  rdfs:isDefinedBy seas:BuildingOntology.    
  
seas:PlusEnergyBuilding a owl:Class ;
  rdfs:label "PlusEnergyBuilding"@en ;
  rdfs:label "Plusenergiatalo"@fi ;  
  rdfs:comment "A net plus-energy building is a building that over a year does generates more energy than it uses. "@en ;
  rdfs:subClassOf seas:Building;
  vs:term_status "testing" ;
  rdfs:isDefinedBy seas:BuildingOntology.    
     
#Building categorization based on occupancy and activities 
#There is no single accepted categorization avilable, some types selected from:
#International building occupancy based categories (USA)
#The Classification of Types of Constructions (EU)
#Finnish building categorization VTJ2000 (Finland)

seas:ResidentalBuilding a owl:Class ;
  rdfs:label "ResidentalBuilding"@en ;
  rdfs:label "Asuinrakennus"@fi ;  
  rdfs:comment "A residential building is a building at least half of which is used for residential purposes. "@en ;
  rdfs:subClassOf seas:Building;
  vs:term_status "testing" ;
  rdfs:isDefinedBy seas:BuildingOntology.   
  
seas:HolidayBuilding a owl:Class ;
  rdfs:label "HolidayBuilding"@en ; 
  rdfs:label "VapaaAjanRakennus"@fi ;  
  rdfs:comment "A secondary residential building used only occasionally during vacations such as a summerhouse or cottage. "@en ;
  rdfs:subClassOf seas:ResidentalBuilding;
  vs:term_status "testing" ;
  rdfs:isDefinedBy seas:BuildingOntology.   
  
seas:NonResidentalBuilding a owl:Class ;
  rdfs:label "NonResidentalBuilding"@en ;
  rdfs:comment "A  non-residential building is a building at least half of which is used for other than residential purposes. "@en ;
  rdfs:subClassOf seas:Building;
  vs:term_status "testing" ;
  rdfs:isDefinedBy seas:BuildingOntology.     

seas:MercantileBuilding a owl:Class ;
  rdfs:label "MercantileBuilding"@en ;
  rdfs:label "Liikerakennus"@fi;  
  rdfs:comment "Places where goods are displayed and sold. Examples: grocery stores, department stores, and gas stations."@en ;
  rdfs:subClassOf seas:NonResidentalBuilding;
  vs:term_status "testing" ;
  rdfs:isDefinedBy seas:BuildingOntology.  
  
seas:OfficeBuilding a owl:Class ;
  rdfs:label "BusinessBuilding"@en ;
  rdfs:label "Toimistorakennus"@fi;  
  rdfs:comment "Places where services are provided. Examples: banks, insurance agencies"@en ;
  rdfs:subClassOf seas:NonResidentalBuilding;
  vs:term_status "testing" ;
  rdfs:isDefinedBy seas:BuildingOntology.    
   
seas:AssemblyBuilding a owl:Class ;
  rdfs:label "AssemblyBuilding"@en ;
  rdfs:label "Kokoontumisrakennus"@fi ;  
  rdfs:comment "places used for people gathering for entertainment, worship, and eating or drinking. Examples: churches, restaurants"@en;
  rdfs:subClassOf seas:NonResidentalBuilding;
  vs:term_status "testing" ;
  rdfs:isDefinedBy seas:BuildingOntology.    

seas:InstitutionalBuilding a owl:Class ;
  rdfs:label "InstitutionalBuilding"@en ;  
  rdfs:label "HoitoalanRakennus"@fi;    
  rdfs:comment "Institutions such as hospitals providing medical and surgical treatment and nursing care for ill or injured people"@en ;
  rdfs:subClassOf seas:NonResidentalBuilding;
  vs:term_status "testing" ;
  rdfs:isDefinedBy seas:BuildingOntology.     
  
seas:EducationalBuilding a owl:Class ;
  rdfs:label "EducationalBuilding"@en ;
  rdfs:label "Opetusrakennus"@fi ;  
  rdfs:comment "Schools and day care centers."@en ;
  rdfs:subClassOf seas:NonResidentalBuilding;
  vs:term_status "testing" ;
  rdfs:isDefinedBy seas:BuildingOntology.      
           
seas:IndustrialBuilding a owl:Class ;
  rdfs:label "IndustrialBuilding"@en ;
  rdfs:comment "Buildings used for industrial production, e.g. factories, workshops, slaughterhouses, breweries, assembly plants, etc."@en ;
  rdfs:subClassOf seas:NonResidentalBuilding;
  vs:term_status "testing" ;
  rdfs:isDefinedBy seas:BuildingOntology.    

seas:PowerplantBuilding a owl:Class ;
  rdfs:label "PowerplantBuilding"@en ;
  rdfs:label "VoimalaRakennus"@fi ;  
  rdfs:comment "Places housing any type of a power plants"@en ;
  rdfs:subClassOf seas:IndustrialBuilding;
  vs:term_status "testing" ;
  rdfs:isDefinedBy seas:BuildingOntology.      
  
seas:StorageBuilding a owl:Class ;
  rdfs:label "StorageBuilding"@en ;
  rdfs:label "VarastoRakennus"@fi ;  
  rdfs:comment "Places where items are stored. Examples: warehouses, reservoirs and silos."@en ;
  rdfs:subClassOf seas:NonResidentalBuilding;
  vs:term_status "testing" ;
  rdfs:isDefinedBy seas:BuildingOntology.    

#Different types of residental buildings
seas:SmallHouse a owl:Class ;
  rdfs:label "SmallHouse"@en ;
  rdfs:label "Pientalo"@en ;  
  rdfs:comment "A detached small residental building"@en ;
  rdfs:subClassOf seas:ResidentalBuilding;
  vs:term_status "testing" ;
  rdfs:isDefinedBy seas:BuildingOntology.   

seas:SmallHouse a owl:Class ;
  rdfs:label "SmallHouse"@en ;
  rdfs:label "Pientalo"@en ;  
  rdfs:comment "A detached small residental building"@en ;
  rdfs:subClassOf seas:ResidentalBuilding;
  vs:term_status "testing" ;
  rdfs:isDefinedBy seas:BuildingOntology.   
  
seas:OneDwellingBuilding a owl:Class ;
  rdfs:label "OneDwellingBuilding"@en ;
  rdfs:label "YhdenAsunnonTalo"@en ;  
  rdfs:comment "Detached house"@en ;
  rdfs:subClassOf seas:SmallHouse;
  vs:term_status "testing" ;
  rdfs:isDefinedBy seas:BuildingOntology.   
  
#Different types of rooms based on their main functional purpose
seas:LivingRoom a owl:Class ;
  rdfs:label "LivingRoom"@en ;
  rdfs:comment "LivingRoom is the main room of daytime activity."@en ;
  rdfs:subClassOf seas:Room;
  vs:term_status "testing" ;
  rdfs:isDefinedBy seas:BuildingOntology.      

seas:Kitchen a owl:Class ;
  rdfs:label "Kitchen"@en ;
  rdfs:comment "Kitchen is a room used mainly for cooking and possibly eating."@en ;
  rdfs:subClassOf seas:Room;
  vs:term_status "testing" ;
  rdfs:isDefinedBy seas:BuildingOntology.      
  
seas:Bedroom a owl:Class ;
  rdfs:label "Bedroom"@en ;
  rdfs:comment "Bedroom is used mainly for sleeping."@en ;
  rdfs:subClassOf seas:Room;
  vs:term_status "testing" ;
  rdfs:isDefinedBy seas:BuildingOntology.   
  
seas:Bathroom a owl:Class ;
  rdfs:label "Bathroom"@en ;
  rdfs:comment "Bathroom is mainly used for bathing &amp; washing up related activities."@en ;
  rdfs:subClassOf seas:Room;
  vs:term_status "testing" ;
  rdfs:isDefinedBy seas:BuildingOntology.      
  
seas:Sauna a owl:Class ;
  rdfs:label "Sauna"@en ;
  rdfs:comment "Sauna is a special type bathroom for enjoying heated steam."@en ;
  rdfs:subClassOf seas:Bathroom;
  vs:term_status "testing" ;
  rdfs:isDefinedBy seas:BuildingOntology.      
  
seas:StorageRoom a owl:Class ;
  rdfs:label "StorageRoom"@en ;
  rdfs:comment "Room for storage."@en ;
  rdfs:subClassOf seas:Room;
  vs:term_status "testing" ;
  rdfs:isDefinedBy seas:BuildingOntology.    
  
seas:Garage a owl:Class ;
  rdfs:label "Garage"@en ;
  rdfs:comment "Room for garage."@en ;
  rdfs:subClassOf seas:Room;
  vs:term_status "testing" ;
  rdfs:isDefinedBy seas:BuildingOntology.     
  
seas:UtilityRoom a owl:Class ;
  rdfs:label "UtilityRoom"@en ;
  rdfs:comment "Room for other special utilities and hobbies."@en ;
  rdfs:subClassOf seas:Room;
  vs:term_status "testing" ;
  rdfs:isDefinedBy seas:BuildingOntology.     
  
seas:Balcony a owl:Class ;
  rdfs:label "Balcony"@en ;
  rdfs:comment "An accessible structure extending from a building, especially outside a window."@en ;
  rdfs:subClassOf seas:BuildingSpace;
  vs:term_status "testing" ;
  rdfs:isDefinedBy seas:BuildingOntology.    

  