# Copyright 2016 ITEA 12004 SEAS Project .
# .
# Licensed under the Apache License, Version 2.0 (the "License") ;
# you may not use this file except in compliance with the License .
# You may obtain a copy of the License a .
# .
#      http://www.apache.org/licenses/LICENSE-2. .
# .
# Unless required by applicable law or agreed to in writing .
# distributed under the License is distributed on an "AS IS" BASIS .
# WITHOUT WARRANTIES OR CONDITIONS OF ANY KIND, either express or implied .
# See the License for the specific language governing permissions an .
# limitations under the License .

@prefix rdf: <http://www.w3.org/1999/02/22-rdf-syntax-ns#> .
@prefix owl: <http://www.w3.org/2002/07/owl#> .
@prefix rdfs: <http://www.w3.org/2000/01/rdf-schema#> .
@prefix xsd: <http://www.w3.org/2001/XMLSchema#> .
@prefix dcterms: <http://purl.org/dc/terms/> .
@prefix vann: <http://purl.org/vocab/vann/> .
@prefix voaf: <http://purl.org/vocommons/voaf#> .
@prefix vs: <http://www.w3.org/2003/06/sw-vocab-status/ns#> .
@prefix qudt: <http://data.qudt.org/qudt/owl/1.0.0/qudt.owl#> .
@prefix cc: <http://creativecommons.org/ns#> .
@prefix foaf: <http://xmlns.com/foaf/0.1/> .
@prefix pep: <https://w3id.org/pep/> .

@prefix seas: <https://w3id.org/seas/> .
@base <https://w3id.org/seas/> .

voaf:Vocabulary a owl:Class .
dcterms:title a owl:AnnotationProperty .
dcterms:description a owl:AnnotationProperty .
dcterms:issued a owl:AnnotationProperty .
dcterms:modified a owl:AnnotationProperty .
dcterms:creator a owl:AnnotationProperty .
dcterms:contributor a owl:AnnotationProperty .
cc:license a owl:AnnotationProperty .
vann:preferredNamespacePrefix a owl:AnnotationProperty .
vann:preferredNamespaceUri a owl:AnnotationProperty .
vs:term_status a owl:AnnotationProperty .
foaf:Person a owl:Class .
foaf:name a owl:DatatypeProperty .


seas:TradingOntology rdf:type voaf:Vocabulary , owl:Ontology ;
  dcterms:title "The SEAS Trading ontology"@en ;
  dcterms:description """The Seas Trading Ontology defines concepts and relations to describe ownership, trading, bilateral contracts and market licenses:

- players own systems and trade commodities, which have a price;
- bilateral electricity contracts are connections between electricity traders at which they exchange
electricity;
- electricity markets are connections between electricity traders at which they exchange electricity,
using a market license;
- electricity markets can be cleared, and balanced;
- evaluations can have a traded volume validity context

  """@en ;
  dcterms:issued "2016-11-15"^^xsd:date ;
  dcterms:modified "2016-11-15"^^xsd:date ;
  dcterms:creator <http://www.maxime-lefrancois.info/me#> ;
  dcterms:contributor <http://www.vtt.fi/JarmoKalaoja> ;
  dcterms:contributor [a foaf:Person ; foaf:name "Antoine Zimmermann" ] ;
  dcterms:contributor [a foaf:Person ; foaf:name "Erkki Siira" ] ;
  dcterms:contributor [a foaf:Person ; foaf:name "Gabriel Santos" ] ;
  cc:license <https://www.apache.org/licenses/LICENSE-2.0> ;
  vann:preferredNamespacePrefix "seas" ;
  vann:preferredNamespaceUri <https://w3id.org/seas/> ;
  owl:imports pep: , seas:PlayerOntology , seas:ElectricPowerSystemOntology , seas:OfferingOntology ;
  owl:versionIRI <https://w3id.org/seas/TradingOntology-1.0> ;
  owl:versionInfo "v1.0" .


seas:owns a owl:ObjectProperty, owl:InverseFunctionalProperty ;
  rdfs:label "owns"@en ;
  rdfs:comment "Links a player to a system it owns."@en ;
  rdfs:domain seas:Player ;
  rdfs:range seas:System ;
  owl:inverseOf seas:isOwnedBy ;
  vs:term_status "testing" ;
  rdfs:isDefinedBy seas:TradingOntology .

seas:isOwnedBy a owl:ObjectProperty , owl:FunctionalProperty ;
  rdfs:label "is owned by"@en ;
  rdfs:comment "Links a system to the one and only player that owns it."@en ;
  rdfs:domain seas:System ;
  rdfs:range seas:Player ;
  owl:inverseOf seas:owns ;
  vs:term_status "testing" ;
  rdfs:isDefinedBy seas:TradingOntology .


seas:trades a owl:ObjectProperty, owl:InverseFunctionalProperty ;
  rdfs:label "trades"@en ;
  rdfs:comment "Links a player to a commodity it trades."@en ;
  rdfs:domain seas:Player ;
  rdfs:range seas:Commodity ;
  owl:inverseOf seas:isTradedBy ;
  vs:term_status "testing" ;
  rdfs:isDefinedBy seas:TradingOntology .

seas:isTradedBy a owl:ObjectProperty , owl:FunctionalProperty ;
  rdfs:label "is traded by"@en ;
  rdfs:comment "Links a commodity to the one and only player that trades it."@en ;
  rdfs:domain seas:Commodity ;
  rdfs:range seas:Player ;
  owl:inverseOf seas:trades ;
  vs:term_status "testing" ;
  rdfs:isDefinedBy seas:TradingOntology .


seas:Commodity a owl:Class ;
  rdfs:label "Commodity"@en ;
  rdfs:comment """In economics, a commodity is a marketable item produced to satisfy wants or needs. Often the item is fungible. Economic commodities comprise goods and services (source: Wikipedia).

For instance, the electric energy outgoing of a certain connection point can be a commodity, and have a price:

```
[] seas:outgoingElectricEnergy  [
  a seas:ElectricEnergyProperty ;
  seas:price [ 
    a seas:Price ;
    seas:evaluation [ 
      a seas:Evaluation ;
      seas:evaluatedValue "200 €"^^xsd:ucum ;
      seas:hasTradedVolumeContext "12 €/MWh"^^xsd:ucum
    ]
  ]
]
``` 

"""@en ;
  rdfs:subClassOf seas:Property ;
  rdfs:subClassOf [ owl:onProperty seas:isPropertyOf ; owl:someValuesFrom seas:ConnectionPoint ] ;
  rdfs:subClassOf [ owl:onProperty seas:price ; owl:someValuesFrom seas:PriceProperty ] ;
  vs:term_status "testing" ;
  rdfs:isDefinedBy seas:TradingOntology .

  seas:Good a owl:Class ;
    rdfs:label "Good"@en ;
    rdfs:comment """In economics, a good is a material that satisfies human wants and provides utility, for example, to a consumer making a purchase while getting an enough-satisfying product. A common distinction is made between 'goods' that are tangible property, and services, which are non-physical (source: Wikipedia)."""@en ;
    rdfs:subClassOf seas:Commodity ;
    owl:disjointWith seas:Service ;
    vs:term_status "testing" ;
    rdfs:isDefinedBy seas:TradingOntology .

  seas:Service a owl:Class ;
    rdfs:label "Service"@en ;
    rdfs:comment """In economics, a service is an economic activity where an immaterial exchange of value occurs. When a service such as labor is performed the buyer does not take exclusive ownership of that which is purchased, unless agreed upon by buyer and seller. The benefits of such a service, if priced, are held to be self-evident in the buyer's willingness to pay for it (source: Wikipedia).
    """@en ;
    rdfs:subClassOf seas:Commodity ;
    owl:disjointWith seas:Good ;
    vs:term_status "testing" ;
    rdfs:isDefinedBy seas:TradingOntology .

    seas:AncillaryService a owl:Class ;
      rdfs:label "Ancillary Service"@en ;
      rdfs:comment """Ancillary services are the specialty services and functions provided by the electric grid that facilitate and support the continuous flow of electricity so that supply will continually meet demand (source: Wikipedia).

    These include black start capability (the ability to restart a grid following a blackout); frequency response (to maintain system frequency with automatic and very fast responses); fast reserve (which can provide additional energy when needed); the provision of reactive power and various other services. (source: Entso-e)"""@en ;
      rdfs:subClassOf seas:Service ;
      vs:term_status "testing" ;
      rdfs:isDefinedBy seas:TradingOntology .


seas:PriceProperty a owl:Class ;
  rdfs:label "Price Property"@en ;
  rdfs:comment """The class of price properties, whose value is expressed using some currency."""@en ;
  rdfs:subClassOf seas:Property ;
  vs:term_status "testing" ;
  rdfs:isDefinedBy seas:TradingOntology .

  seas:NettPriceProperty a owl:Class ;
    rdfs:label "Nett Price Property"@en ;
    rdfs:comment """The class of nett price properties, that have no tax."""@en ;
    rdfs:subClassOf seas:PriceProperty ;
    owl:disjointWith seas:GrossPriceProperty ;
    vs:term_status "testing" ;
    rdfs:isDefinedBy seas:TradingOntology .

  seas:GrossPriceProperty a owl:Class ;
    rdfs:label "Price Property"@en ;
    rdfs:comment """The class of gross price properties, that have some tax.

  A gross price has some properties such as a nett price, and some taxes."""@en ;
    rdfs:subClassOf seas:PriceProperty ;
    owl:disjointWith seas:NettPriceProperty ;
    vs:term_status "testing" ;
    rdfs:isDefinedBy seas:TradingOntology .

seas:price a owl:ObjectProperty , owl:FunctionalProperty ;
  rdfs:label "price"@en ;
  rdfs:comment """The price of some commodity."""@en ;
  rdfs:subPropertyOf seas:hasProperty ;
  rdfs:domain seas:Commodity ;
  rdfs:range seas:PriceProperty ;
  vs:term_status "testing" ;
  rdfs:isDefinedBy seas:TradingOntology .
    
  seas:grossPrice a owl:ObjectProperty , owl:FunctionalProperty ;
    rdfs:label "gross price"@en ;
    rdfs:comment """Links a price property to its gross price, including any taxes."""@en ;
    rdfs:subPropertyOf seas:price ;
    rdfs:range seas:GrossPriceProperty ;
    vs:term_status "testing" ;
    rdfs:isDefinedBy seas:TradingOntology .

  seas:nettPrice a owl:ObjectProperty , owl:FunctionalProperty ;
    rdfs:label "nett price"@en ;
    rdfs:comment """Links a price property to its gross price, excluding any taxes."""@en ;
    rdfs:subPropertyOf seas:price ;
    rdfs:range seas:NettPriceProperty ;
    vs:term_status "testing" ;
    rdfs:isDefinedBy seas:TradingOntology .

  seas:tax a owl:ObjectProperty ;
    rdfs:label "tax"@en ;
    rdfs:comment """Tax for the commodity, quantified as a percentage of something.

Functional sub properties of `seas:tax` must precise what that _something_ is."""@en ;
    rdfs:subPropertyOf seas:hasProperty ;
    rdfs:domain seas:Commodity ;
    vs:term_status "testing" ;
    rdfs:isDefinedBy seas:TradingOntology .

    seas:valueAddedTax a owl:ObjectProperty , owl:FunctionalProperty ;
      rdfs:label "value added tax"@en ;
      rdfs:comment """A value-added tax (VAT), known in some countries as a goods and services tax (GST), is a type of general consumption tax that is collected incrementally, based on the value added, at each stage of production and is usually implemented as a destination-based tax, where the tax rate is based on the location of the customer (source: Wikipedia).

      The value added tax is quantified as a percentage of the nett price."""@en ;
      rdfs:subPropertyOf seas:tax , seas:hasProperty ;
      rdfs:domain seas:Commodity ;
      vs:term_status "testing" ;
      rdfs:isDefinedBy seas:TradingOntology .


seas:operatedBy a owl:ObjectProperty ;
  rdfs:label "operated by"@en ;
  rdfs:comment "Links some connection to a player that regulates what's happening through that connection."@en ;
  rdfs:domain seas:Connection ;
  rdfs:range seas:Player ;
  vs:term_status "testing" ;
  rdfs:isDefinedBy seas:TradingOntology .


seas:tradesElectricityWith a owl:ObjectProperty ;
  rdfs:label "trades electricity with"@en ;
  rdfs:comment """An Electricity Player can trade electricity directly with another electricity player, through an electricity bilateral contract. They then exchange some of the commodities they trade.

These connections are qualified with class `seas:ElectricityBilateralContract`."""@en ;
  rdfs:subPropertyOf seas:connectedTo ;
  rdfs:domain seas:ElectricityTrader ;
  rdfs:range seas:ElectricityTrader ;
  vs:term_status "testing" ;
  rdfs:isDefinedBy seas:TradingOntology .

  seas:ElectricityBilateralContract a owl:Class ;
    rdfs:label "Electricity Bilateral Contract"@en ;
    rdfs:comment """An electricity bilateral contract is both a connection between electricity players, and a contract. It only connects electricity traders.

It is linked to some player that validates each trade."""@en ;
    rdfs:subClassOf seas:Connection , seas:Contract ;
    rdfs:subClassOf [ owl:onProperty seas:connectsSystem ; owl:allValuesFrom seas:ElectricityTrader ] ;
    rdfs:subClassOf [ owl:onProperty seas:operatedBy ; owl:someValuesFrom seas:Player ] ;
    vs:term_status "testing" ;
    rdfs:isDefinedBy seas:TradingOntology .


seas:tradesElectricityOn a owl:ObjectProperty ;
  rdfs:label "trades electricity on"@en ;
  rdfs:comment """An Electricity Player can trade electricity on an Electricity Market.

For example,

```
<http://market.com/> a seas:ElectricityMarket .

<http://agregator.com> a seas:ElectricityTrader ;
  seas:tradesElectricityOn <http://market.com/> .

<http://otheragregator.com> a seas:ElectricityTrader ;
  seas:tradesElectricityOn <http://market.com/> .
```

These connections are qualified with class `seas:ElectricityMarketLicense`.


For example,

```
<http://agregator.com> seas:hasElectricityMarketLicense <http://market.com/license12> .
<http://otheragregator.com> seas:hasElectricityMarketLicense <http://market.com/license32> .

<http://market.com/> seas:connectsSystem <http://agregator.com> , <http://otheragregator.com> .
<http://market.com/> seas:connectsSystemAt <http://market.com/license12> , <http://market.com/license32> .
```

"""@en ;
  rdfs:subPropertyOf seas:connectedThrough ;
  rdfs:domain seas:ElectricityTrader ;
  rdfs:range seas:ElectricityMarket ;
  vs:term_status "testing" ;
  rdfs:isDefinedBy seas:TradingOntology .

  seas:ElectricityMarketLicense a owl:Class ;
    rdfs:label "Electricity Market License"@en ;
    rdfs:comment """An Electricity Market License is a connection point between a player and a market."""@en ;
    rdfs:subClassOf seas:ConnectionPoint ;
    vs:term_status "testing" ;
    rdfs:isDefinedBy seas:TradingOntology .

  seas:hasElectricityMarketLicense a owl:ObjectProperty ;
    rdfs:label "has electricity market license"@en ;
    rdfs:comment """Links an electricity player to its electricity market license."""@en ;
    rdfs:subPropertyOf seas:connectsAt ;
    rdfs:domain seas:ElectricityTrader ;
    rdfs:range seas:ElectricityMarketLicense ;
    vs:term_status "testing" ;
    rdfs:isDefinedBy seas:TradingOntology .

  seas:ElectricityMarket rdfs:subClassOf seas:Connection ;
    rdfs:subClassOf [ owl:onProperty seas:connectsSystem ; owl:allValuesFrom seas:ElectricityTrader ] ;
    rdfs:subClassOf [ owl:onProperty seas:connectsSystemAt ; owl:allValuesFrom seas:ElectricityMarketLicense ] .


seas:Clearing a owl:Class ;
  rdfs:label "Clearing"@en ;
  rdfs:comment """In economics, market clearing is the process by which, in an economic market, the supply of whatever is traded is equated to the demand, so that there is no leftover supply or demand (source: Wikipedia).
  """@en ;
  rdfs:subClassOf pep:Process ;
  vs:term_status "testing" ;
  rdfs:isDefinedBy seas:TradingOntology .

seas:ClearingExecution a owl:Class ;
  rdfs:label "Clearing Execution"@en ;
  rdfs:comment """A process executed by some player. The execution of some clearing process on an electricity market."""@en ;
  rdfs:subClassOf pep:ProcessExecution ;
  rdfs:subClassOf [ owl:onProperty pep:executedBy ; owl:someValuesFrom seas:Player ] ;
  rdfs:subClassOf [ owl:onProperty pep:methodUsed ; owl:someValuesFrom seas:Clearing ] ;
  owl:equivalentClass [ owl:onProperty pep:methodUsed ; owl:someValuesFrom seas:Clearing ] ;
  vs:term_status "testing" ;
  rdfs:isDefinedBy seas:TradingOntology .


seas:Balancing a owl:Class ;
  rdfs:label "Balancing"@en ;
  rdfs:comment "Balancing refers to the process in which a Balance responsible party acts to ensure that demand is equal to supply after markets have closed, in and near real time (source: Entso-e)."@en ;
  rdfs:subClassOf pep:Process ;
  vs:term_status "testing" ;
  rdfs:isDefinedBy seas:TradingOntology .

seas:BalancingExecution a owl:Class ;
  rdfs:label "Balancing Execution"@en ;
  rdfs:comment """The execution of some balancing process on a market."""@en ;
  rdfs:subClassOf pep:ProcessExecution ;
  rdfs:subClassOf [ owl:onProperty pep:executedBy ; owl:someValuesFrom seas:TransmissionSystemOperator ] ;
  rdfs:subClassOf [ owl:onProperty pep:methodUsed ; owl:someValuesFrom seas:Balancing ] ;
  owl:equivalentClass [ owl:onProperty pep:methodUsed ; owl:someValuesFrom seas:Balancing ] ;
  vs:term_status "testing" ;
  rdfs:isDefinedBy seas:TradingOntology .


seas:hasTradedVolumeContext a owl:ObjectProperty , owl:FunctionalProperty ;
  rdfs:label "has traded volume context"@en ;
  rdfs:comment """Links an evaluation to its traded volume validity context.

  for instance .

```
<myConnectionPoint> seas:outgoingElectricEnergy <whatIGive> .

<whatIGive> seas:price <priceOfWhatIGive> .

<priceOfWhatIGive> seas:evaluation <evaluationOfThePriceOfWhatIGive> .

<evaluationOfThePriceOfWhatIGive> a seas:Evaluation ;
  seas:evaluatedValue "200 €"^^cdt:ucum ;
  seas:hasTradedVolumeContext "12 €/MWh"^^cdt:ucum .
```

This concept needs polishing ... please ping me if necessary."""@en ;
  rdfs:subPropertyOf seas:hasValidityContext ;
  rdfs:domain seas:Evaluation ;
  rdfs:range seas:ElectricEnergyProperty ;
  vs:term_status "testing" ;
  rdfs:isDefinedBy seas:TradingOntology .

